add the entire walderfest proof into rocq dir

lean4/rocq/FsubL_alt.v
@@ -1,12 +1,25 @@
 (***************************************************************************
-* Preservation and Progress for System-F with Subtyping - Definitions      *
-* Brian Aydemir & Arthur Charguéraud, March 2007                           *
+  Preservation and Progress for System-F
+  with Subtyping, Bottom and Lower Bounds
+
+- based on the POPLMark solution of
+  Brian Aydemir & Arthur Charguéraud, March 2007
+  cf. https://github.com/samuelgruetter/dot-calculus/blob/master/ln/Fsub_Definitions.v
+  cf. https://github.com/samuelgruetter/dot-calculus/blob/master/ln/Fsub_Infrastructure.v
+  cf. https://github.com/samuelgruetter/dot-calculus/blob/master/ln/Fsub_Part1A.v
+
+- compared to FsubL, does push back on values, using possible types
+
 ***************************************************************************)
 
 Set Implicit Arguments.
 Require Import LibLN.
 Implicit Types x : var.
 Implicit Types X : var.
+
+(***************************************************************************
+* Definitions                                                              *
+***************************************************************************)
 
 (* ********************************************************************** *)
 (** * Description of the Language *)
@@ -15,10 +28,11 @@ Implicit Types X : var.
 
 Inductive typ : Set :=
   | typ_top   : typ
+  | typ_bot   : typ
   | typ_bvar  : nat -> typ
   | typ_fvar  : var -> typ
   | typ_arrow : typ -> typ -> typ
-  | typ_all   : typ -> typ -> typ.
+  | typ_all   : typ -> typ -> typ -> typ.
 
 (** Representation of pre-terms *)
 
@@ -27,7 +41,7 @@ Inductive trm : Set :=
   | trm_fvar : var -> trm
   | trm_abs  : typ -> trm -> trm
   | trm_app  : trm -> trm -> trm
-  | trm_tabs : typ -> trm -> trm
+  | trm_tabs : typ -> typ -> trm -> trm
   | trm_tapp : trm -> typ -> trm.
 
 (** Opening up a type binder occuring in a type *)
@@ -35,10 +49,11 @@ Inductive trm : Set :=
 Fixpoint open_tt_rec (K : nat) (U : typ) (T : typ) {struct T} : typ :=
   match T with
   | typ_top         => typ_top
+  | typ_bot         => typ_bot
   | typ_bvar J      => If K = J then U else (typ_bvar J)
   | typ_fvar X      => typ_fvar X
   | typ_arrow T1 T2 => typ_arrow (open_tt_rec K U T1) (open_tt_rec K U T2)
-  | typ_all T1 T2   => typ_all (open_tt_rec K U T1) (open_tt_rec (S K) U T2)
+  | typ_all T0 T1 T2   => typ_all (open_tt_rec K U T0) (open_tt_rec K U T1) (open_tt_rec (S K) U T2)
   end.
 
 Definition open_tt T U := open_tt_rec 0 U T.
@@ -51,7 +66,7 @@ Fixpoint open_te_rec (K : nat) (U : typ) (e : trm) {struct e} : trm :=
   | trm_fvar x    => trm_fvar x
   | trm_abs V e1  => trm_abs  (open_tt_rec K U V)  (open_te_rec K U e1)
   | trm_app e1 e2 => trm_app  (open_te_rec K U e1) (open_te_rec K U e2)
-  | trm_tabs V e1 => trm_tabs (open_tt_rec K U V)  (open_te_rec (S K) U e1)
+  | trm_tabs VS VU e1 => trm_tabs (open_tt_rec K U VS) (open_tt_rec K U VU)  (open_te_rec (S K) U e1)
   | trm_tapp e1 V => trm_tapp (open_te_rec K U e1) (open_tt_rec K U V)
   end.
 
@@ -65,7 +80,7 @@ Fixpoint open_ee_rec (k : nat) (f : trm) (e : trm) {struct e} : trm :=
   | trm_fvar x    => trm_fvar x
   | trm_abs V e1  => trm_abs V (open_ee_rec (S k) f e1)
   | trm_app e1 e2 => trm_app (open_ee_rec k f e1) (open_ee_rec k f e2)
-  | trm_tabs V e1 => trm_tabs V (open_ee_rec k f e1)
+  | trm_tabs VS VU e1 => trm_tabs VS VU (open_ee_rec k f e1)
   | trm_tapp e1 V => trm_tapp (open_ee_rec k f e1) V
   end.
 
@@ -82,16 +97,19 @@ Notation "t 'open_ee_var' x" := (open_ee t (trm_fvar x)) (at level 67).
 Inductive type : typ -> Prop :=
   | type_top :
       type typ_top
+  | type_bot :
+      type typ_bot
   | type_var : forall X,
       type (typ_fvar X)
   | type_arrow : forall T1 T2,
       type T1 ->
       type T2 ->
       type (typ_arrow T1 T2)
-  | type_all : forall L T1 T2,
+  | type_all : forall L T0 T1 T2,
+      type T0 ->
       type T1 ->
       (forall X, X \notin L -> type (T2 open_tt_var X)) ->
-      type (typ_all T1 T2).
+      type (typ_all T0 T1 T2).
 
 (** Terms as locally closed pre-terms *)
 
@@ -106,27 +124,21 @@ Inductive term : trm -> Prop :=
       term e1 ->
       term e2 ->
       term (trm_app e1 e2)
-  | term_tabs : forall L V e1,
-      type V ->
+  | term_tabs : forall L VS VU e1,
+      type VS ->
+      type VU ->
       (forall X, X \notin L -> term (e1 open_te_var X)) ->
-      term (trm_tabs V e1)
+      term (trm_tabs VS VU e1)
   | term_tapp : forall e1 V,
       term e1 ->
       type V ->
       term (trm_tapp e1 V).
 
-(** Binding are either mapping type or term variables.
- [X ~<: T] is a subtyping asumption and [x ~: T] is
- a typing assumption *)
+(** Binding are either mapping type or term variables. *)
 
 Inductive bind : Set :=
-  | bind_sub : typ -> bind
+  | bind_sub : typ -> typ -> bind
   | bind_typ : typ -> bind.
-
-Notation "X ~<: T" := (X ~ bind_sub T)
-  (at level 23, left associativity) : env_scope.
-Notation "x ~: T" := (x ~ bind_typ T)
-  (at level 23, left associativity) : env_scope.
 
 (** Environment is an associative list of bindings. *)
 
@@ -140,18 +152,21 @@ Definition env := LibEnv.env bind.
 Inductive wft : env -> typ -> Prop :=
   | wft_top : forall E,
       wft E typ_top
-  | wft_var : forall U E X,
-      binds X (bind_sub U) E ->
+  | wft_bot : forall E,
+      wft E typ_bot
+  | wft_var : forall T0 T1 E X,
+      binds X (bind_sub T0 T1) E ->
       wft E (typ_fvar X)
   | wft_arrow : forall E T1 T2,
       wft E T1 ->
       wft E T2 ->
       wft E (typ_arrow T1 T2)
-  | wft_all : forall L E T1 T2,
+  | wft_all : forall L E T0 T1 T2,
+      wft E T0 ->
       wft E T1 ->
       (forall X, X \notin L ->
-        wft (E & X ~<: T1) (T2 open_tt_var X)) ->
-      wft E (typ_all T1 T2).
+        wft (E & X ~ bind_sub T0 T1) (T2 open_tt_var X)) ->
+      wft E (typ_all T0 T1 T2).
 
 (** A environment E is well-formed if it contains no duplicate bindings
   and if each type in it is well-formed with respect to the environment
@@ -160,10 +175,10 @@ Inductive wft : env -> typ -> Prop :=
 Inductive okt : env -> Prop :=
   | okt_empty :
       okt empty
-  | okt_sub : forall E X T,
-      okt E -> wft E T -> X # E -> okt (E & X ~<: T)
+  | okt_sub : forall E X T0 T1,
+      okt E -> wft E T0 -> wft E T1 -> X # E -> okt (E & X ~ bind_sub T0 T1)
   | okt_typ : forall E x T,
-      okt E -> wft E T -> x # E -> okt (E & x ~: T).
+      okt E -> wft E T -> x # E -> okt (E & x ~ bind_typ T).
 
 (** Subtyping relation *)
 
@@ -172,23 +187,37 @@ Inductive sub : env -> typ -> typ -> Prop :=
       okt E ->
       wft E S ->
       sub E S typ_top
+  | sub_bot : forall E T,
+      okt E ->
+      wft E T ->
+      sub E typ_bot T
   | sub_refl_tvar : forall E X,
       okt E ->
       wft E (typ_fvar X) ->
       sub E (typ_fvar X) (typ_fvar X)
-  | sub_trans_tvar : forall U E T X,
-      binds X (bind_sub U) E ->
-      sub E U T ->
-      sub E (typ_fvar X) T
+  | sub_tvar : forall T0 T1 E X,
+      okt E ->
+      binds X (bind_sub T0 T1) E ->
+      sub E (typ_fvar X) T1
+  | sub_tvar_lower : forall T0 T1 E X,
+      okt E ->
+      binds X (bind_sub T0 T1) E ->
+      sub E T0 (typ_fvar X)
   | sub_arrow : forall E S1 S2 T1 T2,
       sub E T1 S1 ->
       sub E S2 T2 ->
       sub E (typ_arrow S1 S2) (typ_arrow T1 T2)
-  | sub_all : forall L E S1 S2 T1 T2,
+  | sub_all : forall L E S0 S1 S2 T0 T1 T2,
+      sub E S0 T0 ->
       sub E T1 S1 ->
       (forall X, X \notin L ->
-          sub (E & X ~<: T1) (S2 open_tt_var X) (T2 open_tt_var X)) ->
-      sub E (typ_all S1 S2) (typ_all T1 T2).
+          sub (E & X ~ bind_sub T0 T1) (S2 open_tt_var X) (T2 open_tt_var X)) ->
+      sub E (typ_all S0 S1 S2) (typ_all T0 T1 T2)
+  | sub_trans : forall E S T U,
+      sub E S T ->
+      sub E T U ->
+      sub E S U
+.
 
 (** Typing relation *)
 
@@ -199,18 +228,19 @@ Inductive typing : env -> trm -> typ -> Prop :=
       typing E (trm_fvar x) T
   | typing_abs : forall L E V e1 T1,
       (forall x, x \notin L ->
-        typing (E & x ~: V) (e1 open_ee_var x) T1) ->
+        typing (E & x ~ bind_typ V) (e1 open_ee_var x) T1) ->
       typing E (trm_abs V e1) (typ_arrow V T1)
   | typing_app : forall T1 E e1 e2 T2,
       typing E e1 (typ_arrow T1 T2) ->
       typing E e2 T1 ->
       typing E (trm_app e1 e2) T2
-  | typing_tabs : forall L E V e1 T1,
+  | typing_tabs : forall L E VS VU e1 T1,
       (forall X, X \notin L ->
-        typing (E & X ~<: V) (e1 open_te_var X) (T1 open_tt_var X)) ->
-      typing E (trm_tabs V e1) (typ_all V T1)
-  | typing_tapp : forall T1 E e1 T T2,
-      typing E e1 (typ_all T1 T2) ->
+        typing (E & X ~ bind_sub VS VU) (e1 open_te_var X) (T1 open_tt_var X)) ->
+      typing E (trm_tabs VS VU e1) (typ_all VS VU T1)
+  | typing_tapp : forall T0 T1 E e1 T T2,
+      typing E e1 (typ_all T0 T1 T2) ->
+      sub E T0 T ->
       sub E T T1 ->
       typing E (trm_tapp e1 T) (open_tt T2 T)
   | typing_sub : forall S E e T,
@@ -223,8 +253,8 @@ Inductive typing : env -> trm -> typ -> Prop :=
 Inductive value : trm -> Prop :=
   | value_abs  : forall V e1, term (trm_abs V e1) ->
                  value (trm_abs V e1)
-  | value_tabs : forall V e1, term (trm_tabs V e1) ->
-                 value (trm_tabs V e1).
+  | value_tabs : forall VS VU e1, term (trm_tabs VS VU e1) ->
+                 value (trm_tabs VS VU e1).
 
 (** One-step reduction *)
 
@@ -245,17 +275,17 @@ Inductive red : trm -> trm -> Prop :=
       term (trm_abs V e1) ->
       value v2 ->
       red (trm_app (trm_abs V e1) v2) (open_ee e1 v2)
-  | red_tabs : forall V1 e1 V2,
-      term (trm_tabs V1 e1) ->
+  | red_tabs : forall V0 V1 e1 V2,
+      term (trm_tabs V0 V1 e1) ->
       type V2 ->
-      red (trm_tapp (trm_tabs V1 e1) V2) (open_te e1 V2).
+      red (trm_tapp (trm_tabs V0 V1 e1) V2) (open_te e1 V2).
 
 (** Our goal is to prove preservation and progress *)
 
-Definition preservation := forall E e e' T,
-  typing E e T ->
+Definition preservation := forall e e' T,
+  typing empty e T ->
   red e e' ->
-  typing E e' T.
+  typing empty e' T.
 
 Definition progress := forall e T,
   typing empty e T ->
@@ -263,7 +293,7 @@ Definition progress := forall e T,
   \/ exists e', red e e'.
 
 (***************************************************************************
-* Preservation and Progress for System-F with Subtyping - Infrastructure   *
+* Infrastructure                                                           *
 ***************************************************************************)
 
 (* ********************************************************************** *)
@@ -274,10 +304,11 @@ Definition progress := forall e T,
 Fixpoint fv_tt (T : typ) {struct T} : vars :=
   match T with
   | typ_top         => \{}
+  | typ_bot         => \{}
   | typ_bvar J      => \{}
   | typ_fvar X      => \{X}
   | typ_arrow T1 T2 => (fv_tt T1) \u (fv_tt T2)
-  | typ_all T1 T2   => (fv_tt T1) \u (fv_tt T2)
+  | typ_all T0 T1 T2   => (fv_tt T0) \u (fv_tt T1) \u (fv_tt T2)
   end.
 
 (** Computing free type variables in a term *)
@@ -288,7 +319,7 @@ Fixpoint fv_te (e : trm) {struct e} : vars :=
   | trm_fvar x    => \{}
   | trm_abs V e1  => (fv_tt V) \u (fv_te e1)
   | trm_app e1 e2 => (fv_te e1) \u (fv_te e2)
-  | trm_tabs V e1 => (fv_tt V) \u (fv_te e1)
+  | trm_tabs VS VU e1 => (fv_tt VS) \u (fv_tt VU) \u (fv_te e1)
   | trm_tapp e1 V => (fv_tt V) \u (fv_te e1)
   end.
 
@@ -300,7 +331,7 @@ Fixpoint fv_ee (e : trm) {struct e} : vars :=
   | trm_fvar x    => \{x}
   | trm_abs V e1  => (fv_ee e1)
   | trm_app e1 e2 => (fv_ee e1) \u (fv_ee e2)
-  | trm_tabs V e1 => (fv_ee e1)
+  | trm_tabs VS VU e1 => (fv_ee e1)
   | trm_tapp e1 V => (fv_ee e1)
   end.
 
@@ -309,10 +340,11 @@ Fixpoint fv_ee (e : trm) {struct e} : vars :=
 Fixpoint subst_tt (Z : var) (U : typ) (T : typ) {struct T} : typ :=
   match T with
   | typ_top         => typ_top
+  | typ_bot         => typ_bot
   | typ_bvar J      => typ_bvar J
   | typ_fvar X      => If X = Z then U else (typ_fvar X)
   | typ_arrow T1 T2 => typ_arrow (subst_tt Z U T1) (subst_tt Z U T2)
-  | typ_all T1 T2   => typ_all (subst_tt Z U T1) (subst_tt Z U T2)
+  | typ_all T0 T1 T2   => typ_all (subst_tt Z U T0) (subst_tt Z U T1) (subst_tt Z U T2)
   end.
 
 (** Substitution for free type variables in terms. *)
@@ -323,7 +355,7 @@ Fixpoint subst_te (Z : var) (U : typ) (e : trm) {struct e} : trm :=
   | trm_fvar x    => trm_fvar x
   | trm_abs V e1  => trm_abs  (subst_tt Z U V)  (subst_te Z U e1)
   | trm_app e1 e2 => trm_app  (subst_te Z U e1) (subst_te Z U e2)
-  | trm_tabs V e1 => trm_tabs (subst_tt Z U V)  (subst_te Z U e1)
+  | trm_tabs VS VU e1 => trm_tabs (subst_tt Z U VS) (subst_tt Z U VU)  (subst_te Z U e1)
   | trm_tapp e1 V => trm_tapp (subst_te Z U e1) (subst_tt Z U V)
   end.
 
@@ -335,7 +367,7 @@ Fixpoint subst_ee (z : var) (u : trm) (e : trm) {struct e} : trm :=
   | trm_fvar x    => If x = z then u else (trm_fvar x)
   | trm_abs V e1  => trm_abs V (subst_ee z u e1)
   | trm_app e1 e2 => trm_app (subst_ee z u e1) (subst_ee z u e2)
-  | trm_tabs V e1 => trm_tabs V (subst_ee z u e1)
+  | trm_tabs VS VU e1 => trm_tabs VS VU (subst_ee z u e1)
   | trm_tapp e1 V => trm_tapp (subst_ee z u e1) V
   end.
 
@@ -343,7 +375,7 @@ Fixpoint subst_ee (z : var) (u : trm) (e : trm) {struct e} : trm :=
 
 Definition subst_tb (Z : var) (P : typ) (b : bind) : bind :=
   match b with
-  | bind_sub T => bind_sub (subst_tt Z P T)
+  | bind_sub T0 T1 => bind_sub (subst_tt Z P T0) (subst_tt Z P T1)
   | bind_typ T => bind_typ (subst_tt Z P T)
   end.
 
@@ -355,7 +387,7 @@ Definition subst_tb (Z : var) (P : typ) (b : bind) : bind :=
 Hint Constructors type term wft ok okt value red.
 
 Hint Resolve
-  sub_top sub_refl_tvar sub_arrow
+  sub_top sub_bot sub_refl_tvar sub_arrow
   typing_var typing_app typing_tapp typing_sub.
 
 (** Gathering free names already used in the proofs *)
@@ -405,12 +437,19 @@ Tactic Notation "apply_empty" "*" constr(F) :=
 
 (** Tactic to undo when Coq does too much simplification *)
 
-Ltac unsimpl_map_bind :=
+Ltac unsimpl_map_bind_sub :=
+  match goal with |- context [ ?B (subst_tt ?Z ?P ?U0) (subst_tt ?Z ?P ?U1) ] =>
+    unsimpl ((subst_tb Z P) (B U0 U1)) end.
+
+Ltac unsimpl_map_bind_typ :=
   match goal with |- context [ ?B (subst_tt ?Z ?P ?U) ] =>
     unsimpl ((subst_tb Z P) (B U)) end.
 
-Tactic Notation "unsimpl_map_bind" "*" :=
-  unsimpl_map_bind; auto*.
+Tactic Notation "unsimpl_map_bind_sub" "*" :=
+  unsimpl_map_bind_sub; auto*.
+
+Tactic Notation "unsimpl_map_bind_typ" "*" :=
+  unsimpl_map_bind_typ; auto*.
 
 
 (* ********************************************************************** *)
@@ -696,76 +735,98 @@ Proof.
   intros. gen_eq K: (E & G). gen E F G.
   induction H; intros; subst; eauto.
   (* case: var *)
-  apply (@wft_var U). apply* binds_weaken.
+  apply (@wft_var T0 T1). apply* binds_weaken.
   (* case: all *)
-  apply_fresh* wft_all as Y. apply_ih_bind* H1.
+  apply_fresh* wft_all as Y. apply_ih_bind* H2.
+Qed.
+
+Lemma wft_weaken_empty : forall T F,
+  wft empty T ->
+  ok F ->
+  wft F T.
+Proof.
+  intros. lets A: (@wft_weaken empty T empty F).
+  repeat rewrite concat_empty_r in *. repeat rewrite concat_empty_l in *.
+  apply* A.
 Qed.
 
 (** Through narrowing *)
 
-Lemma wft_narrow : forall V F U T E X,
-  wft (E & X ~<: V & F) T ->
-  ok (E & X ~<: U & F) ->
-  wft (E & X ~<: U & F) T.
+Lemma wft_narrow : forall V0 V1 F U0 U1 T E X,
+  wft (E & X ~ bind_sub V0 V1 & F) T ->
+  ok (E & X ~ bind_sub U0 U1 & F) ->
+  wft (E & X ~ bind_sub U0 U1 & F) T.
 Proof.
-  intros. gen_eq K: (E & X ~<: V & F). gen E F.
+  intros. gen_eq K: (E & X ~ bind_sub V0 V1 & F). gen E F.
   induction H; intros; subst; eauto.
   destruct (binds_middle_inv H) as [K|[K|K]]; try destructs K.
     applys wft_var. apply* binds_concat_right.
     subst. applys wft_var. apply~ binds_middle_eq.
     applys wft_var. apply~ binds_concat_left.
      apply* binds_concat_left.
-  apply_fresh* wft_all as Y. apply_ih_bind* H1.
+  apply_fresh* wft_all as Y. apply_ih_bind* H2.
 Qed.
 
 (** Through strengthening *)
 
 Lemma wft_strengthen : forall E F x U T,
- wft (E & x ~: U & F) T -> wft (E & F) T.
+ wft (E & x ~ bind_typ U & F) T -> wft (E & F) T.
 Proof.
-  intros. gen_eq G: (E & x ~: U & F). gen F.
+  intros. gen_eq G: (E & x ~ bind_typ U & F). gen F.
   induction H; intros F EQ; subst; auto.
-  apply* (@wft_var U0).
+  apply* (@wft_var T0 T1).
   destruct (binds_concat_inv H) as [?|[? ?]].
     apply~ binds_concat_right.
     destruct (binds_push_inv H1) as [[? ?]|[? ?]].
       subst. false.
       apply~ binds_concat_left.
   (* todo: binds_cases tactic *)
-  apply_fresh* wft_all as Y. apply_ih_bind* H1.
+  apply_fresh* wft_all as Y. apply_ih_bind* H2.
 Qed.
 
 (** Through type substitution *)
 
-Lemma wft_subst_tb : forall F Q E Z P T,
-  wft (E & Z ~<: Q & F) T ->
+Lemma wft_subst_tb : forall F Q0 Q1 E Z P T,
+  wft (E & Z ~ bind_sub Q0 Q1 & F) T ->
   wft E P ->
   ok (E & map (subst_tb Z P) F) ->
   wft (E & map (subst_tb Z P) F) (subst_tt Z P T).
 Proof.
-  introv WT WP. gen_eq G: (E & Z ~<: Q & F). gen F.
+  introv WT WP. gen_eq G: (E & Z ~ bind_sub Q0 Q1 & F). gen F.
   induction WT; intros F EQ Ok; subst; simpl subst_tt; auto.
   case_var*.
     apply_empty* wft_weaken.
     destruct (binds_concat_inv H) as [?|[? ?]].
-      apply (@wft_var (subst_tt Z P U)).
+      apply (@wft_var (subst_tt Z P T0) (subst_tt Z P T1)).
        apply~ binds_concat_right.
-       unsimpl_map_bind. apply~ binds_map.
+       unsimpl_map_bind_sub. apply binds_map.
+       assumption.
       destruct (binds_push_inv H1) as [[? ?]|[? ?]].
         subst. false~.
         applys wft_var. apply* binds_concat_left.
   apply_fresh* wft_all as Y.
-   unsimpl ((subst_tb Z P) (bind_sub T1)).
+   unsimpl ((subst_tb Z P) (bind_sub T0 T1)).
    lets: wft_type.
    rewrite* subst_tt_open_tt_var.
    apply_ih_map_bind* H0.
 Qed.
 
+Lemma wft_subst_tb_empty : forall F Q0 Q1 Z P T,
+  wft (Z ~ bind_sub Q0 Q1 & F) T ->
+  wft empty P ->
+  ok (map (subst_tb Z P) F) ->
+  wft (map (subst_tb Z P) F) (subst_tt Z P T).
+Proof.
+  intros.
+  lets A: (@wft_subst_tb F Q0 Q1 empty Z P T).
+  repeat rewrite concat_empty_l in *. apply* A.
+Qed.
+
 (** Through type reduction *)
 
-Lemma wft_open : forall E U T1 T2,
+Lemma wft_open : forall E U T0 T1 T2,
   ok E ->
-  wft E (typ_all T1 T2) ->
+  wft E (typ_all T0 T1 T2) ->
   wft E U ->
   wft E (open_tt T2 U).
 Proof.
@@ -792,8 +853,8 @@ Hint Extern 1 (ok _) => apply ok_from_okt.
 
 (** Extraction from a subtyping assumption in a well-formed environments *)
 
-Lemma wft_from_env_has_sub : forall x U E,
-  okt E -> binds x (bind_sub U) E -> wft E U.
+Lemma wft_from_env_has_sub : forall x U0 U1 E,
+  okt E -> binds x (bind_sub U0 U1) E -> wft E U0 /\ wft E U1.
 Proof.
   induction E using env_ind; intros Ok B.
   false* binds_empty_inv.
@@ -801,12 +862,12 @@ Proof.
     false (empty_push_inv H0).
     destruct (eq_push_inv H) as [? [? ?]]. subst. clear H.
      destruct (binds_push_inv B) as [[? ?]|[? ?]]. subst.
-       inversions H3. apply_empty* wft_weaken.
-       apply_empty* wft_weaken.
+       inversions H4. split; apply_empty* wft_weaken.
+       split; apply_empty* wft_weaken.
     destruct (eq_push_inv H) as [? [? ?]]. subst. clear H.
      destruct (binds_push_inv B) as [[? ?]|[? ?]]. subst.
        inversions H3.
-       apply_empty* wft_weaken.
+       split; apply_empty* wft_weaken.
 Qed.
 
 (** Extraction from a typing assumption in a well-formed environments *)
@@ -820,7 +881,7 @@ Proof.
     false (empty_push_inv H0).
     destruct (eq_push_inv H) as [? [? ?]]. subst. clear H.
      destruct (binds_push_inv B) as [[? ?]|[? ?]]. subst.
-       inversions H3.
+       inversions H4.
        apply_empty* wft_weaken.
     destruct (eq_push_inv H) as [? [? ?]]. subst. clear H.
      destruct (binds_push_inv B) as [[? ?]|[? ?]]. subst.
@@ -831,7 +892,7 @@ Qed.
 (** Extraction from a well-formed environment *)
 
 Lemma wft_from_okt_typ : forall x T E,
-  okt (E & x ~: T) -> wft E T.
+  okt (E & x ~ bind_typ T) -> wft E T.
 Proof.
   intros. inversions* H.
   false (empty_push_inv H1).
@@ -839,12 +900,12 @@ Proof.
   destruct (eq_push_inv H0) as [? [? ?]]. inversions~ H4.
 Qed.
 
-Lemma wft_from_okt_sub : forall x T E,
-  okt (E & x ~<: T) -> wft E T.
+Lemma wft_from_okt_sub : forall x T0 T1 E,
+  okt (E & x ~ bind_sub T0 T1) -> wft E T0 /\ wft E T1.
 Proof.
   intros. inversions* H.
   false (empty_push_inv H1).
-  destruct (eq_push_inv H0) as [? [? ?]]. inversions~ H4.
+  destruct (eq_push_inv H0) as [? [? ?]]. inversions~ H5.
   destruct (eq_push_inv H0) as [? [? ?]]. false.
 Qed.
 
@@ -861,7 +922,7 @@ Qed.
 Hint Resolve wft_weaken_right.
 Hint Resolve wft_from_okt_typ wft_from_okt_sub.
 Hint Immediate wft_from_env_has_sub wft_from_env_has_typ.
-Hint Resolve wft_subst_tb.
+Hint Resolve wft_subst_tb wft_subst_tb_empty.
 
 
 (* ********************************************************************** *)
@@ -870,7 +931,7 @@ Hint Resolve wft_subst_tb.
 (** Inversion lemma *)
 
 Lemma okt_push_inv : forall E X B,
-  okt (E & X ~ B) -> exists T, B = bind_sub T \/ B = bind_typ T.
+  okt (E & X ~ B) -> (exists T0 T1, B = bind_sub T0 T1) \/ (exists T, B = bind_typ T).
 Proof.
   introv O. inverts O.
     false* empty_push_inv.
@@ -878,8 +939,8 @@ Proof.
     lets (?&?&?): (eq_push_inv H). subst*.
 Qed.
 
-Lemma okt_push_sub_inv : forall E X T,
-  okt (E & X ~<: T) -> okt E /\ wft E T /\ X # E.
+Lemma okt_push_sub_inv : forall E X T0 T1,
+  okt (E & X ~ bind_sub T0 T1) -> okt E /\ wft E T0 /\ wft E T1 /\ X # E.
 Proof.
   introv O. inverts O.
     false* empty_push_inv.
@@ -887,12 +948,12 @@ Proof.
     lets (?&?&?): (eq_push_inv H). false.
 Qed.
 
-Lemma okt_push_sub_type : forall E X T,
-  okt (E & X ~<: T) -> type T.
-Proof. intros. applys wft_type. forwards*: okt_push_sub_inv. Qed.
+Lemma okt_push_sub_type : forall E X T0 T1,
+  okt (E & X ~ bind_sub T0 T1) -> type T0 /\ type T1.
+Proof. intros. split; applys wft_type; forwards*: okt_push_sub_inv. Qed.
 
 Lemma okt_push_typ_inv : forall E x T,
-  okt (E & x ~: T) -> okt E /\ wft E T /\ x # E.
+  okt (E & x ~ bind_typ T) -> okt E /\ wft E T /\ x # E.
 Proof.
   introv O. inverts O.
     false* empty_push_inv.
@@ -901,24 +962,24 @@ Proof.
 Qed.
 
 Lemma okt_push_typ_type : forall E X T,
-  okt (E & X ~: T) -> type T.
+  okt (E & X ~ bind_typ T) -> type T.
 Proof. intros. applys wft_type. forwards*: okt_push_typ_inv. Qed.
 
 Hint Immediate okt_push_sub_type okt_push_typ_type.
 
 (** Through narrowing *)
 
-Lemma okt_narrow : forall V (E F:env) U X,
-  okt (E & X ~<: V & F) ->
-  wft E U ->
-  okt (E & X ~<: U & F).
+Lemma okt_narrow : forall V0 V1 (E F:env) U0 U1 X,
+  okt (E & X ~ bind_sub V0 V1 & F) ->
+  wft E U0 -> wft E U1 ->
+  okt (E & X ~ bind_sub U0 U1 & F).
 Proof.
-  introv O W. induction F using env_ind.
+  introv O W0 W1. induction F using env_ind.
   rewrite concat_empty_r in *. lets*: (okt_push_sub_inv O).
   rewrite concat_assoc in *.
-   lets (T&[?|?]): okt_push_inv O; subst.
-     lets (?&?&?): (okt_push_sub_inv O).
-      applys~ okt_sub. applys* wft_narrow.
+   lets [[T0 [T1 Hsub]] | [T Htyp]]: (okt_push_inv O); subst.
+     lets (?&?&?&?): (okt_push_sub_inv O).
+      applys~ okt_sub; applys* wft_narrow.
      lets (?&?&?): (okt_push_typ_inv O).
       applys~ okt_typ. applys* wft_narrow.
 Qed.
@@ -926,23 +987,23 @@ Qed.
 (** Through strengthening *)
 
 Lemma okt_strengthen : forall x T (E F:env),
-  okt (E & x ~: T & F) ->
+  okt (E & x ~ bind_typ T & F) ->
   okt (E & F).
 Proof.
  introv O. induction F using env_ind.
   rewrite concat_empty_r in *. lets*: (okt_push_typ_inv O).
   rewrite concat_assoc in *.
-   lets (U&[?|?]): okt_push_inv O; subst.
-     lets (?&?&?): (okt_push_sub_inv O).
-      applys~ okt_sub. applys* wft_strengthen.
+   lets [[U0 [U1 Hsub]] | [U Htyp]]: (okt_push_inv O); subst.
+     lets (?&?&?&?): (okt_push_sub_inv O).
+      applys~ okt_sub; applys* wft_strengthen.
      lets (?&?&?): (okt_push_typ_inv O).
       applys~ okt_typ. applys* wft_strengthen.
 Qed.
 
 (** Through type substitution *)
 
-Lemma okt_subst_tb : forall Q Z P (E F:env),
-  okt (E & Z ~<: Q & F) ->
+Lemma okt_subst_tb : forall Q0 Q1 Z P (E F:env),
+  okt (E & Z ~ bind_sub Q0 Q1 & F) ->
   wft E P ->
   okt (E & map (subst_tb Z P) F).
 Proof.
@@ -950,16 +1011,26 @@ Proof.
   rewrite map_empty. rewrite concat_empty_r in *.
    lets*: (okt_push_sub_inv O).
   rewrite map_push. rewrite concat_assoc in *.
-   lets (U&[?|?]): okt_push_inv O; subst.
-     lets (?&?&?): (okt_push_sub_inv O).
-      applys~ okt_sub. applys* wft_subst_tb.
+   lets [[U0 [U1 Hsub]] | [U Htyp]]: (okt_push_inv O); subst.
+     lets (?&?&?&?): (okt_push_sub_inv O).
+      applys~ okt_sub; applys* wft_subst_tb.
      lets (?&?&?): (okt_push_typ_inv O).
       applys~ okt_typ. applys* wft_subst_tb.
 Qed.
 
+Lemma okt_subst_tb_empty : forall Q0 Q1 Z P (F:env),
+  okt (Z ~ bind_sub Q0 Q1 & F) ->
+  wft empty P ->
+  okt (map (subst_tb Z P) F).
+Proof.
+  intros.
+  lets A: (@okt_subst_tb Q0 Q1 Z P empty F).
+  repeat rewrite concat_empty_l in *. apply* A.
+Qed.
+
 (** Automation *)
 
-Hint Resolve okt_narrow okt_subst_tb wft_weaken.
+Hint Resolve okt_narrow okt_subst_tb okt_subst_tb_empty wft_weaken.
 Hint Immediate okt_strengthen.
 
 
@@ -973,13 +1044,14 @@ Proof.
  introv. unfold open_tt. generalize 0.
  induction T; simpl; intros k Fr; auto.
  specializes IHT1 k. specializes IHT2 k. auto.
- specializes IHT1 k. specializes IHT2 (S k). auto.
+ specializes IHT1 k. specializes IHT2 k. specializes IHT3 (S k). auto.
 Qed.
 
 Lemma notin_fv_wf : forall E X T,
   wft E T -> X # E -> X \notin fv_tt T.
 Proof.
   induction 1; intros Fr; simpl.
+  eauto.
   eauto.
   rewrite notin_singleton. intro. subst. applys binds_fresh_inv H Fr.
   notin_simpl; auto.
@@ -991,7 +1063,9 @@ Lemma map_subst_tb_id : forall G Z P,
 Proof.
   induction 1; intros Fr; autorewrite with rew_env_map; simpl.
   auto.
-  rewrite* <- IHokt. rewrite* subst_tt_fresh. apply* notin_fv_wf.
+  rewrite* <- IHokt.
+    rewrite* subst_tt_fresh. rewrite* subst_tt_fresh.
+    apply* notin_fv_wf. apply* notin_fv_wf.
   rewrite* <- IHokt. rewrite* subst_tt_fresh. apply* notin_fv_wf.
 Qed.
 
@@ -1004,10 +1078,18 @@ Qed.
 Lemma sub_regular : forall E S T,
   sub E S T -> okt E /\ wft E S /\ wft E T.
 Proof.
-  induction 1. auto*. auto*. auto*. jauto_set; auto. (* auto* too slow *)
-  split. auto*. split;
-   apply_fresh* wft_all as Y;
-    forwards~: (H1 Y); apply_empty* (@wft_narrow T1).
+  induction 1. auto*. auto*. auto*.
+  splits*. eapply proj2. apply* wft_from_env_has_sub.
+  splits*. eapply proj1. apply* wft_from_env_has_sub.
+  jauto_set; auto. (* auto* too slow *)
+  split. auto*.
+   inversion IHsub1 as [_ [HwfS0 HwfT0]].
+   inversion IHsub2 as [_ [HwfT1 HwfS1]].
+   split;
+   apply_fresh wft_all as Y; try assumption;
+   forwards~: (H2 Y);
+   apply_empty* (@wft_narrow T0 T1).
+  auto*.
 Qed.
 
 (** The typing relation is restricted to well-formed objects. *)
@@ -1035,15 +1117,21 @@ Proof.
    apply_fresh* term_tabs as y.
      pick_fresh y. forwards~ K: (H0 y). destructs K.
        forwards*: okt_push_sub_inv.
+       inversion H4 as [_ [Hwf _]]. apply wft_type with (E:=E). assumption.
+     pick_fresh y. forwards~ K: (H0 y). destructs K.
+       forwards*: okt_push_sub_inv.
+       inversion H4 as [_ [_ [Hwf _]]]. apply wft_type with (E:=E). assumption.
      forwards~ K: (H0 y). destructs K. auto.
    apply_fresh* wft_all as Y.
+     pick_fresh y. forwards~ K: (H0 y). destructs K.
+      forwards*: okt_push_sub_inv.
      pick_fresh y. forwards~ K: (H0 y). destructs K.
       forwards*: okt_push_sub_inv.
      forwards~ K: (H0 Y). destructs K.
       forwards*: okt_push_sub_inv.
   splits*; destructs (sub_regular H0).
    apply* term_tapp. applys* wft_type.
-   applys* wft_open T1.
+   applys* wft_open T0 T1.
   splits*. destructs~ (sub_regular H0).
 Qed.
 
@@ -1096,7 +1184,7 @@ Hint Extern 1 (term ?e) =>
   end.
 
 (***************************************************************************
-* Preservation and Progress for System-F with Subtyping - Proofs           *
+* Proofs                                                                   *
 ***************************************************************************)
 
 (** In parentheses are given the label of the corresponding
@@ -1128,10 +1216,24 @@ Lemma sub_weakening : forall E F G S T,
    sub (E & F & G) S T.
 Proof.
   introv Typ. gen F. inductions Typ; introv Ok; auto.
-  (* case: fvar trans *)
-  apply* sub_trans_tvar. apply* binds_weaken.
+  (* case: fvar *)
+  apply* sub_tvar. apply* binds_weaken.
+  (* case: fvar lower *)
+  apply* sub_tvar_lower. apply* binds_weaken.
   (* case: all *)
   apply_fresh* sub_all as Y. apply_ih_bind* H0.
+  (* case: trans *)
+  apply* sub_trans.
+Qed.
+
+Lemma sub_weakening_empty : forall F G S T,
+   sub G S T ->
+   okt (F & G) ->
+   sub (F & G) S T.
+Proof.
+  intros.
+  lets A: (@sub_weakening empty F G S T).
+  repeat rewrite concat_empty_l in *. apply* A.
 Qed.
 
 (* ********************************************************************** *)
@@ -1139,65 +1241,66 @@ Qed.
 
 Section NarrowTrans.
 
-Definition transitivity_on Q := forall E S T,
-  sub E S Q -> sub E Q T -> sub E S T.
-
-Hint Unfold transitivity_on.
-
 Hint Resolve wft_narrow.
 
-Lemma sub_narrowing_aux : forall Q F E Z P S T,
-  transitivity_on Q ->
-  sub (E & Z ~<: Q & F) S T ->
-  sub E P Q ->
-  sub (E & Z ~<: P & F) S T.
+Lemma sub_narrowing_aux : forall Q0 Q1 F E Z P0 P1 S T,
+  sub (E & Z ~ bind_sub Q0 Q1 & F) S T ->
+  sub E Q0 P0 ->
+  sub E P1 Q1 ->
+  sub (E & Z ~ bind_sub P0 P1 & F) S T.
 Proof.
-  introv TransQ SsubT PsubQ.
+  introv SsubT Q0subP0 P1subQ1.
   inductions SsubT; introv.
   apply* sub_top.
+  apply* sub_bot.
   apply* sub_refl_tvar.
   tests EQ: (X = Z).
-    lets M: (@okt_narrow Q).
-    apply (@sub_trans_tvar P).
-      asserts~ N: (ok (E & Z ~<: P & F)).
+  lets M: (@okt_narrow Q0 Q1).
+    apply binds_middle_eq_inv in H0. inversion H0. subst.
+    apply sub_trans with (T:=P1).
+      apply* sub_tvar.
+       asserts~ N: (ok (E & Z ~ bind_sub P0 P1 & F)).
        lets: ok_middle_inv_r N.
        apply~ binds_middle_eq.
-      apply TransQ.
-        do_rew* concat_assoc (apply_empty* sub_weakening).
-        binds_get H. auto*.
-    apply* (@sub_trans_tvar U). binds_cases H; auto.
+      do_rew* concat_assoc (apply_empty* sub_weakening). auto*.
+    apply* sub_tvar. instantiate (1:=T0). binds_cases H0; auto*.
+  tests EQ: (X = Z).
+    lets M: (@okt_narrow Q0 Q1).
+    apply binds_middle_eq_inv in H0. inversion H0. subst.
+    apply sub_trans with (T:=P0).
+      do_rew* concat_assoc (apply_empty* sub_weakening).
+      apply* sub_tvar_lower.
+       asserts~ N: (ok (E & Z ~ bind_sub P0 P1 & F)).
+       lets: ok_middle_inv_r N.
+       apply~ binds_middle_eq.
+      auto*.
+    apply* sub_tvar_lower. instantiate (1:=T1). binds_cases H0; auto*.
   apply* sub_arrow.
-  apply_fresh* sub_all as Y. apply_ih_bind* H0.
+  apply_fresh* sub_all as Y. apply_ih_bind H0. auto. auto. auto. auto.
+  apply sub_trans with (T:=T). apply* IHSsubT1. apply* IHSsubT2.
 Qed.
 
-Lemma sub_transitivity : forall Q,
-  transitivity_on Q.
-Proof.
-  intro Q. introv SsubQ QsubT. asserts* W: (type Q).
-  gen E S T. set_eq Q' EQ: Q. gen Q' EQ.
-  induction W; intros Q' EQ E S SsubQ;
-    induction SsubQ; try discriminate; inversions EQ;
-      intros T QsubT; inversions keep QsubT;
-        eauto 4 using sub_trans_tvar.
-  (* case: all / top -> only needed to fix well-formedness,
-     by building back what has been deconstructed too much *)
-  assert (sub E (typ_all S1 S2) (typ_all T1 T2)).
-    apply_fresh* sub_all as y.
-  auto*.
-  (* case: all / all *)
-  apply_fresh sub_all as Y. auto*.
-  applys~ (H0 Y). lets: (IHW T1).
-  apply_empty* (@sub_narrowing_aux T1).
-Qed.
-
-Lemma sub_narrowing : forall Q E F Z P S T,
-  sub E P Q ->
-  sub (E & Z ~<: Q & F) S T ->
-  sub (E & Z ~<: P & F) S T.
+Lemma sub_narrowing : forall Q0 Q1 E F Z P0 P1 S T,
+  sub E Q0 P0 ->
+  sub E P1 Q1 ->
+  sub (E & Z ~ bind_sub Q0 Q1 & F) S T ->
+  sub (E & Z ~ bind_sub P0 P1 & F) S T.
 Proof.
   intros.
   apply* sub_narrowing_aux.
-  apply* sub_transitivity.
+Qed.
+
+Lemma sub_narrowing_empty : forall Q0 Q1 Z P0 P1 S T,
+  sub empty Q0 P0 ->
+  sub empty P1 Q1 ->
+  sub (Z ~ bind_sub Q0 Q1) S T ->
+  sub (Z ~ bind_sub P0 P1) S T.
+Proof.
+  intros.
+  rewrite <- (concat_empty_r (Z ~ bind_sub P0 P1)).
+  rewrite <- (concat_empty_l (Z ~ bind_sub P0 P1)).
+  eapply sub_narrowing; eauto.
+  rewrite concat_empty_r. rewrite concat_empty_l. auto.
 Qed.
 
 End NarrowTrans.
@@ -1205,34 +1308,58 @@ End NarrowTrans.
 (* ********************************************************************** *)
 (** Type substitution preserves subtyping (10) *)
 
-Lemma sub_through_subst_tt : forall Q E F Z S T P,
-  sub (E & Z ~<: Q & F) S T ->
-  sub E P Q ->
+Lemma sub_through_subst_tt : forall Q0 Q1 E F Z S T P,
+  sub (E & Z ~ bind_sub Q0 Q1 & F) S T ->
+  sub E Q0 P ->
+  sub E P Q1 ->
   sub (E & map (subst_tb Z P) F) (subst_tt Z P S) (subst_tt Z P T).
 Proof.
-  introv SsubT PsubQ.
+  introv SsubT Q0subP PsubQ1. lets R: (sub_regular Q0subP).
+  destruct R as [_ [_ Pwf]].
   inductions SsubT; introv; simpl subst_tt.
-  apply* sub_top.
-  case_var.
+  - apply* sub_top.
+  - apply* sub_bot.
+  - case_var.
     apply* sub_reflexivity.
     apply* sub_reflexivity.
-     inversions H0. binds_cases H3.
-      apply* (@wft_var U).
-      apply* (@wft_var (subst_tt Z P U)). unsimpl_map_bind*.
-   case_var.
-    apply (@sub_transitivity Q).
+    inversions H0. binds_cases H3.
+      apply* (@wft_var T0 T1).
+      apply* (@wft_var (subst_tt Z P T0) (subst_tt Z P T1)). unsimpl_map_bind_sub*.
+  - case_var.
+    apply sub_trans with (T:=Q1).
       apply_empty* sub_weakening.
-      rewrite* <- (@subst_tt_fresh Z P Q).
-        binds_get H. auto*.
+      rewrite* <- (@subst_tt_fresh Z P Q1).
+        binds_get H0. inversion H1. subst.
+        apply* sub_reflexivity. apply_empty* wft_weaken.
+        rewrite* subst_tt_fresh.
         apply* (@notin_fv_wf E).
-    apply* (@sub_trans_tvar (subst_tt Z P U)).
+        apply* (@notin_fv_wf E).
+    eapply sub_tvar. auto*. instantiate (1:=subst_tt Z P T0).
       rewrite* (@map_subst_tb_id E Z P).
-        binds_cases H; unsimpl_map_bind*.
-  apply* sub_arrow.
-  apply_fresh* sub_all as X.
-   unsimpl (subst_tb Z P (bind_sub T1)).
-   do 2 rewrite* subst_tt_open_tt_var.
-   apply_ih_map_bind* H0.
+      binds_cases H0; unsimpl_map_bind_sub*.
+  - case_var.
+    apply sub_trans with (T:=Q0).
+      apply_empty* sub_weakening.
+      rewrite* <- (@subst_tt_fresh Z P Q0).
+        binds_get H0. inversion H1. subst.
+        apply* sub_reflexivity.
+        rewrite* subst_tt_fresh.
+        apply* (@notin_fv_wf E).
+        apply* (@notin_fv_wf E).
+        apply_empty* sub_weakening.
+    eapply sub_tvar_lower. auto*. instantiate (1:=subst_tt Z P T1).
+      rewrite* (@map_subst_tb_id E Z P).
+      binds_cases H0; unsimpl_map_bind_sub*.
+  - apply* sub_arrow.
+  - apply_fresh* sub_all as X.
+    unsimpl (subst_tb Z P (bind_sub T0 T1)).
+    repeat rewrite* subst_tt_open_tt_var.
+    assert (E & map (subst_tb Z P) F & X ~ subst_tb Z P (bind_sub T0 T1) =
+            E & map (subst_tb Z P) (F & X ~ bind_sub T0 T1)) as A. {
+      rewrite map_concat. rewrite map_single. rewrite concat_assoc. reflexivity.
+    }
+    rewrite A. eapply H0; eauto. rewrite concat_assoc. reflexivity.
+  - apply* sub_trans.
 Qed.
 
 (* ********************************************************************** *)
@@ -1253,7 +1380,12 @@ Proof.
   apply* typing_app.
   apply_fresh* typing_tabs as X. forwards~ K: (H X).
    apply_ih_bind (H0 X); eauto.
-  apply* typing_tapp. apply* sub_weakening.
+   apply typing_regular in K.
+   inversion K as [HOK _].
+   apply wft_from_okt_sub in HOK.
+   inversion HOK as [HS HU].
+   apply okt_sub; auto.
+  apply* typing_tapp; apply* sub_weakening.
   apply* typing_sub. apply* sub_weakening.
 Qed.
 
@@ -1261,40 +1393,60 @@ Qed.
 (** Strengthening (6) *)
 
 Lemma sub_strengthening : forall x U E F S T,
-  sub (E & x ~: U & F) S T ->
+  sub (E & x ~ bind_typ U & F) S T ->
   sub (E & F) S T.
 Proof.
   intros x U E F S T SsubT.
   inductions SsubT; introv; auto* wft_strengthen.
-  (* case: fvar trans *)
-  apply* (@sub_trans_tvar U0). binds_cases H; auto*.
+  (* case: tvar *)
+  apply* sub_tvar. instantiate (1:=T0). binds_cases H0; auto*.
+  (* case: tvar lower *)
+  apply* sub_tvar_lower. instantiate (1:=T1). binds_cases H0; auto*.
   (* case: all *)
   apply_fresh* sub_all as X. apply_ih_bind* H0.
+  (* case: trans *)
+  apply* sub_trans.
 Qed.
 
 (************************************************************************ *)
 (** Preservation by Type Narrowing (7) *)
 
-Lemma typing_narrowing : forall Q E F X P e T,
-  sub E P Q ->
-  typing (E & X ~<: Q & F) e T ->
-  typing (E & X ~<: P & F) e T.
+Lemma typing_narrowing : forall Q0 Q1 E F X P0 P1 e T,
+  sub E Q0 P0 ->
+  sub E P1 Q1 ->
+  sub E P0 P1 ->
+  typing (E & X ~ bind_sub Q0 Q1 & F) e T ->
+  typing (E & X ~ bind_sub P0 P1 & F) e T.
 Proof.
-  introv PsubQ Typ. gen_eq E': (E & X ~<: Q & F). gen F.
+  introv Q0subP0 P1subQ1 P0subP1 Typ. gen_eq E': (E & X ~ bind_sub Q0 Q1 & F). gen F.
   inductions Typ; introv EQ; subst; simpl.
   binds_cases H0; apply* typing_var.
   apply_fresh* typing_abs as y. apply_ih_bind* H0.
   apply* typing_app.
   apply_fresh* typing_tabs as Y. apply_ih_bind* H0.
-  apply* typing_tapp. apply* (@sub_narrowing Q).
-  apply* typing_sub. apply* (@sub_narrowing Q).
+  apply* typing_tapp; apply* (@sub_narrowing Q0 Q1).
+  apply* typing_sub. apply* (@sub_narrowing Q0 Q1).
+Qed.
+
+Lemma typing_narrowing_empty : forall Q0 Q1 X P0 P1 e T,
+  sub empty Q0 P0 ->
+  sub empty P1 Q1 ->
+  sub empty P0 P1 ->
+  typing (X ~ bind_sub Q0 Q1) e T ->
+  typing (X ~ bind_sub P0 P1) e T.
+Proof.
+  intros.
+  rewrite <- (concat_empty_r (X ~ bind_sub P0 P1)).
+  rewrite <- (concat_empty_l (X ~ bind_sub P0 P1)).
+  eapply typing_narrowing; eauto.
+  rewrite concat_empty_r. rewrite concat_empty_l. auto.
 Qed.
 
 (************************************************************************ *)
 (** Preservation by Term Substitution (8) *)
 
 Lemma typing_through_subst_ee : forall U E F x T e u,
-  typing (E & x ~: U & F) e T ->
+  typing (E & x ~ bind_typ U & F) e T ->
   typing E u U ->
   typing (E & F) (subst_ee x u e) T.
 Proof.
@@ -1309,35 +1461,45 @@ Proof.
   apply_fresh* typing_tabs as Y.
     rewrite* subst_ee_open_te_var.
     apply_ih_bind* H0.
-  apply* typing_tapp. apply* sub_strengthening.
+  apply* typing_tapp; apply* sub_strengthening.
   apply* typing_sub. apply* sub_strengthening.
 Qed.
 
 (************************************************************************ *)
 (** Preservation by Type Substitution (11) *)
 
-Lemma typing_through_subst_te : forall Q E F Z e T P,
-  typing (E & Z ~<: Q & F) e T ->
-  sub E P Q ->
+Lemma typing_through_subst_te : forall Q0 Q1 E F Z e T P,
+  typing (E & Z ~ bind_sub Q0 Q1 & F) e T ->
+  sub E Q0 P ->
+  sub E P Q1 ->
   typing (E & map (subst_tb Z P) F) (subst_te Z P e) (subst_tt Z P T).
 Proof.
-  introv Typ PsubQ.
+  introv Typ Q0subP PsubQ1.
   inductions Typ; introv; simpls subst_tt; simpls subst_te.
-  apply* typing_var. rewrite* (@map_subst_tb_id E Z P).
-   binds_cases H0; unsimpl_map_bind*.
-  apply_fresh* typing_abs as y.
+  - apply* typing_var. rewrite* (@map_subst_tb_id E Z P).
+    binds_cases H0; unsimpl_map_bind_typ*.
+  - apply_fresh* typing_abs as y.
     unsimpl (subst_tb Z P (bind_typ V)).
     rewrite* subst_te_open_ee_var.
-    apply_ih_map_bind* H0.
-  apply* typing_app.
-  apply_fresh* typing_tabs as Y.
-    unsimpl (subst_tb Z P (bind_sub V)).
+    assert (E & map (subst_tb Z P) F & y ~ subst_tb Z P (bind_typ V)=
+            E & map (subst_tb Z P) (F & y ~ bind_typ V)) as A. {
+      rewrite map_concat. rewrite map_single. rewrite concat_assoc. reflexivity.
+    }
+    rewrite A. eapply H0; eauto. rewrite concat_assoc. reflexivity.
+  - apply* typing_app.
+  - apply_fresh* typing_tabs as Y.
+    unsimpl (subst_tb Z P (bind_sub VS VU)).
     rewrite* subst_te_open_te_var.
     rewrite* subst_tt_open_tt_var.
-    apply_ih_map_bind* H0.
-  rewrite* subst_tt_open_tt. apply* typing_tapp.
+    assert (E & map (subst_tb Z P) F & Y ~ subst_tb Z P (bind_sub VS VU)=
+            E & map (subst_tb Z P) (F & Y ~ bind_sub VS VU)) as A. {
+      rewrite map_concat. rewrite map_single. rewrite concat_assoc. reflexivity.
+    }
+    rewrite A. eapply H0; eauto. rewrite concat_assoc. reflexivity.
+  - rewrite* subst_tt_open_tt. apply* typing_tapp.
     apply* sub_through_subst_tt.
-  apply* typing_sub. apply* sub_through_subst_tt.
+    apply* sub_through_subst_tt.
+  - apply* typing_sub. apply* sub_through_subst_tt.
 Qed.
 
 (* ********************************************************************** *)
@@ -1346,33 +1508,113 @@ Qed.
 (* ********************************************************************** *)
 (** Inversions for Typing (13) *)
 
-Lemma typing_inv_abs : forall E S1 e1 T,
-  typing E (trm_abs S1 e1) T ->
-  forall U1 U2, sub E T (typ_arrow U1 U2) ->
-     sub E U1 S1
-  /\ exists S2, exists L, forall x, x \notin L ->
-     typing (E & x ~: S1) (e1 open_ee_var x) S2 /\ sub E S2 U2.
+Inductive possible_types : trm -> typ -> Prop :=
+| pt_top : forall v, value v -> possible_types v typ_top
+| pt_arrow : forall L V V' e1 T1 T1',
+  (forall x, x \notin L -> typing (x ~ bind_typ V) (e1 open_ee_var x) T1) ->
+  sub empty V' V ->
+  sub empty T1 T1' ->
+  possible_types (trm_abs V e1) (typ_arrow V' T1')
+| pt_all : forall L VS VS' VU VU' e1 T1 T1',
+  (forall X, X \notin L -> typing (X ~ bind_sub VS VU) (e1 open_te_var X) (T1 open_tt_var X)) ->
+  sub empty VS VS' ->
+  sub empty VU' VU ->
+  (forall X, X \notin L -> sub (X ~ bind_sub VS' VU') (T1 open_tt_var X) (T1' open_tt_var X)) ->
+  possible_types (trm_tabs VS VU e1) (typ_all VS' VU' T1')
+.
+
+Lemma possible_types_value : forall p T,
+  possible_types p T ->
+  value p.
 Proof.
-  introv Typ. gen_eq e: (trm_abs S1 e1). gen S1 e1.
-  induction Typ; intros S1 b1 EQ U1 U2 Sub; inversions EQ.
-  inversions* Sub. auto* (@sub_transitivity T).
+  introv Hpt. induction Hpt; eauto.
+  - apply value_abs. apply_fresh* term_abs as y.
+    assert (y \notin L) as Fr by auto.
+    specialize (H y Fr). apply typing_regular in H. auto*.
+  - apply value_tabs. apply_fresh* term_tabs as Y.
+    assert (Y \notin L) as Fr by auto.
+    specialize (H Y Fr). apply typing_regular in H. auto*.
 Qed.
 
-Lemma typing_inv_tabs : forall E S1 e1 T,
-  typing E (trm_tabs S1 e1) T ->
-  forall U1 U2, sub E T (typ_all U1 U2) ->
-     sub E U1 S1
-  /\ exists S2, exists L, forall X, X \notin L ->
-     typing (E & X ~<: U1) (e1 open_te_var X) (S2 open_tt_var X)
-     /\ sub (E & X ~<: U1) (S2 open_tt_var X) (U2 open_tt_var X).
+Lemma possible_types_closure : forall v T U,
+  possible_types v T ->
+  sub empty T U ->
+  possible_types v U.
 Proof.
-  intros E S1 e1 T H. gen_eq e: (trm_tabs S1 e1). gen S1 e1.
-  induction H; intros S1 b EQ U1 U2 Sub; inversion EQ.
-  inversions Sub. splits. auto.
-   exists T1. let L1 := gather_vars in exists L1.
-   intros Y Fr. splits.
-    apply_empty* (@typing_narrowing S1). auto.
-  auto* (@sub_transitivity T).
+  introv Hpt Hsub. remember empty as E. gen HeqE. generalize dependent v.
+  induction Hsub; intros; subst; eauto;
+  try solve [false; apply* binds_empty_inv].
+  - apply pt_top. apply* possible_types_value.
+  - inversion Hpt.
+  - inversion Hpt; subst. apply_fresh* pt_arrow as y.
+    eapply sub_trans; eassumption. eapply sub_trans; eassumption.
+  - inversion Hpt; subst. apply_fresh* pt_all as Y.
+    eapply sub_trans; eassumption. eapply sub_trans; eassumption.
+    eapply sub_trans.
+      eapply sub_narrowing_empty. eassumption. eassumption. auto*.
+      assert (Y \notin L) as Fr by auto. specialize (H Y Fr).
+      rewrite concat_empty_l in H. apply H.
+Qed.
+
+Lemma possible_types_typing : forall v T,
+  typing empty v T -> value v ->
+  possible_types v T.
+Proof.
+  introv Ht Hv.
+  remember Ht as Hc. clear HeqHc.
+  remember empty as E. generalize HeqE. generalize Hc.
+  induction Ht; intros; subst; eauto; try solve [inversion Hv].
+  - eapply typing_regular in Hc. destruct Hc as [? [? Hc]].
+    inversion Hc; subst.
+    apply_fresh pt_arrow as y.
+    assert (y \notin L) as Fr by eauto.
+    specialize (H y Fr). rewrite concat_empty_l in H. eapply H.
+    eapply sub_reflexivity; eauto. eapply sub_reflexivity; eauto.
+  - eapply typing_regular in Hc. destruct Hc as [? [? Hc]].
+    inversion Hc; subst.
+    apply_fresh pt_all as Y.
+    assert (Y \notin L) as Fr by eauto.
+    specialize (H Y Fr). rewrite concat_empty_l in H. eapply H.
+    eapply sub_reflexivity; eauto. eapply sub_reflexivity; eauto.
+    eapply sub_reflexivity; eauto.
+    rewrite <- concat_empty_l. eauto.
+    assert (Y \notin L0) as Fr by eauto.
+    specialize (H9 Y Fr). rewrite concat_empty_l in H9. eapply H9.
+  - eapply possible_types_closure; eauto.
+Qed.
+
+Lemma typing_inv_abs : forall S1 e1 T,
+  typing empty (trm_abs S1 e1) T ->
+  forall U1 U2, sub empty T (typ_arrow U1 U2) ->
+     sub empty U1 S1
+  /\ exists S2, exists L, forall x, x \notin L ->
+     typing (x ~ bind_typ S1) (e1 open_ee_var x) S2 /\ sub empty S2 U2.
+Proof.
+  introv Typ Hsub.
+  apply possible_types_typing in Typ; eauto.
+  assert (possible_types (trm_abs S1 e1) (typ_arrow U1 U2)) as Hc. {
+    eapply possible_types_closure; eauto.
+  }
+  inversion Hc; subst.
+  repeat eexists; eauto.
+Qed.
+
+Lemma typing_inv_tabs : forall S10 S11 e1 T,
+  typing empty (trm_tabs S10 S11 e1) T ->
+  forall U10 U11 U2, sub empty T (typ_all U10 U11 U2) -> sub empty U10 U11 ->
+     sub empty S10 U10 /\ sub empty U11 S11
+  /\ exists S2, exists L, forall X, X \notin L ->
+     typing (X ~ bind_sub U10 U11) (e1 open_te_var X) (S2 open_tt_var X)
+     /\ sub (X ~ bind_sub U10 U11) (S2 open_tt_var X) (U2 open_tt_var X).
+Proof.
+  introv Typ Hsub.
+  apply possible_types_typing in Typ; eauto.
+  assert (possible_types (trm_tabs S10 S11 e1) (typ_all U10 U11 U2)) as Hc. {
+    eapply possible_types_closure; eauto.
+  }
+  inversion Hc; subst.
+  repeat eexists; eauto.
+  eapply typing_narrowing_empty; eauto.
 Qed.
 
 (* ********************************************************************** *)
@@ -1380,8 +1622,9 @@ Qed.
 
 Lemma preservation_result : preservation.
 Proof.
-  introv Typ. gen e'. induction Typ; introv Red;
-   try solve [ inversion Red ].
+  introv Typ. gen_eq E: (@empty bind). gen e'.
+  induction Typ; introv QEQ; introv Red;
+   try solve [inversion Typ; congruence]; try solve [ inversion Red ].
   (* case: app *)
   inversions Red; try solve [ apply* typing_app ].
   destruct~ (typing_inv_abs Typ1 (U1:=T1) (U2:=T2)) as [P1 [S2 [L P2]]].
@@ -1389,20 +1632,20 @@ Proof.
     pick_fresh X. forwards~ K: (P2 X). destruct K.
      rewrite* (@subst_ee_intro X).
      apply_empty (@typing_through_subst_ee V).
-       apply* (@typing_sub S2). apply_empty* sub_weakening.
+       apply* (@typing_sub S2). rewrite concat_empty_l. auto*. apply_empty* sub_weakening_empty.
        auto*.
   (* case: tapp *)
   inversions Red; try solve [ apply* typing_tapp ].
-  destruct~ (typing_inv_tabs Typ (U1:=T1) (U2:=T2)) as [P1 [S2 [L P2]]].
-    apply* sub_reflexivity.
+  destruct~ (typing_inv_tabs Typ (U10:=T0) (U11:=T1) (U2:=T2)) as [P1 [S20 [S21 [L P2]]]].
+    apply* sub_reflexivity. apply sub_trans with (T:=T); eauto.
     pick_fresh X. forwards~ K: (P2 X). destruct K.
      rewrite* (@subst_te_intro X).
      rewrite* (@subst_tt_intro X).
-     (* todo: apply empty here *)
-     asserts_rewrite (E = E & map (subst_tb X T) empty).
-       rewrite map_empty. rewrite~ concat_empty_r.
-     apply* (@typing_through_subst_te T1).
-       rewrite* concat_empty_r.
+     rewrite <- (@concat_empty_l bind (@empty bind)).
+     erewrite <- map_empty at 2.
+     apply* (@typing_through_subst_te T0 T1).
+     rewrite concat_empty_r. rewrite concat_empty_l.
+     apply* typing_sub.
   (* case sub *)
   apply* typing_sub.
 Qed.
@@ -1413,30 +1656,32 @@ Qed.
 (* ********************************************************************** *)
 (** Canonical Forms (14) *)
 
+Lemma value_not_bot : forall t T,
+  value t -> typing empty t T -> T <> typ_bot.
+Proof.
+  introv Val Typ.
+  eapply possible_types_typing in Typ; eauto.
+  inversion Typ; congruence.
+Qed.
+
 Lemma canonical_form_abs : forall t U1 U2,
   value t -> typing empty t (typ_arrow U1 U2) ->
   exists V, exists e1, t = trm_abs V e1.
 Proof.
-  introv Val Typ. gen_eq E: (@empty bind).
-  gen_eq T: (typ_arrow U1 U2). gen U1 U2.
-  induction Typ; introv EQT EQE;
-   try solve [ inversion Val | inversion EQT | eauto ].
-    subst. inversion H.
-      false (binds_empty_inv H0).
-      inversions H0. forwards*: IHTyp.
+  introv Val Typ.
+  apply possible_types_typing in Typ; eauto.
+  inversion Typ; subst.
+  repeat eexists; eauto.
 Qed.
 
-Lemma canonical_form_tabs : forall t U1 U2,
-  value t -> typing empty t (typ_all U1 U2) ->
-  exists V, exists e1, t = trm_tabs V e1.
+Lemma canonical_form_tabs : forall t U0 U1 U2,
+  value t -> typing empty t (typ_all U0 U1 U2) ->
+  exists V0 V1, exists e1, t = trm_tabs V0 V1 e1.
 Proof.
-  introv Val Typ. gen_eq E: (@empty bind).
-  gen_eq T: (typ_all U1 U2). gen U1 U2.
-  induction Typ; introv EQT EQE;
-   try solve [ inversion Val | inversion EQT | eauto ].
-    subst. inversion H.
-      false* binds_empty_inv.
-      inversions H0. forwards*: IHTyp.
+  introv Val Typ.
+  apply possible_types_typing in Typ; eauto.
+  inversion Typ; subst.
+  repeat eexists; eauto.
 Qed.
 
 (* ********************************************************************** *)
@@ -1459,10 +1704,9 @@ Proof.
   left*.
   (* case: tapp *)
   right. destruct~ IHTyp as [Val1 | [e1' Rede1']].
-    destruct (canonical_form_tabs Val1 Typ) as [S [e3 EQ]].
+    destruct (canonical_form_tabs Val1 Typ) as [S0 [S1 [e3 EQ]]].
       subst. exists* (open_te e3 T).
       exists* (trm_tapp e1' T).
   (* case: sub *)
   auto*.
 Qed.
-
